messageInvariantPrototypes/toylock/types.dfy
@@ -1,0 +1,20 @@
+include "../lib/MonotonicityLibrary.dfy"
+
+module Types {
+  import opened UtilitiesLibrary
+
+  type HostId = nat
+  type UniqueKey = int
+
+  datatype Message = Grant(src: nat, dst: HostId, epoch: nat) {
+    ghost function Src() : nat {
+      src
+    }
+
+    ghost function Dst() : nat {
+      dst
+    }
+  }
+
+  datatype MessageOps = MessageOps(recv:Option<Message>, send:Option<Message>)
+} // end module Types
